still no merge

TestTheories/Sorting.thy
@@ -23,10 +23,10 @@ fun qsort :: "nat list \<Rightarrow> nat list" where
 | "qsort (t # ts) = (qsort [r <- ts. r \<le> t]) @ [t] @ (qsort [r <- ts. \<not> (r \<le> t)])"
 
 
-fun sorted' :: "nat list \<Rightarrow> bool" where
-  "sorted' []                   = True"
-| "sorted' [x]         = True"
-| "sorted' (r # (t # ts))  = (r \<le> t \<and> sorted' (t # ts))"
+fun sorted2 :: "nat list \<Rightarrow> bool" where
+  "sorted2 []                   = True"
+| "sorted2 [x]         = True"
+| "sorted2 (r # (t # ts))  = (r \<le> t \<and> sorted2 (t # ts))"
 
 fun merge :: "nat list \<Rightarrow> nat list \<Rightarrow> nat list" where
   "merge rs [] = rs"
@@ -40,44 +40,68 @@ fun msort :: "nat list => nat list" where
 | "msort ts = merge (msort (List.take (length ts div 2) ts)) (* size instead? *)
                     (msort (List.drop (length ts div 2) ts))"
 
-(* lemma sortCons: "r \<le> t \<and> sorted' (t # ts) \<Longrightarrow> sorted' (r # (t # ts))" by simp *)
+(* lemma sortCons: "r \<le> t \<and> sorted2 (t # ts) \<Longrightarrow> sorted2 (r # (t # ts))" by simp *)
 
-lemma mer1: "sorted' ts \<Longrightarrow> sorted' (merge [] ts)"
-(*by(metis sorted'.cases merge.simps)*) (* replace of cases by inductions *)
+lemma mer1[thy_expl]: "sorted2 ts \<Longrightarrow> sorted2 (merge [] ts)"
+(*by(metis sorted2.cases merge.simps)*) (* replace of cases by inductions *)
 by hipster_induct_simp_metis
 
-lemma mer2: "sorted' ts \<Longrightarrow> sorted' (merge [t] ts)" (* sorted'.induct! *)
+lemma mer2[thy_expl]: "sorted2 ts \<Longrightarrow> sorted2 (merge [t] ts)" (* sorted2.induct! *)
 by hipster_induct_schemes
 
-lemma mer3: "sorted' ts \<Longrightarrow> sorted' (merge ts [t])" (* sorted'.induct! *)
+lemma mer3[thy_expl]: "sorted2 ts \<Longrightarrow> sorted2 (merge ts [t])" (* sorted2.induct! *)
 by hipster_induct_schemes
 
-lemma mer4: "sorted' (t # ts) \<and> \<not> t \<le> r \<Longrightarrow> sorted' (r # (merge (t#ts) []))" by simp
+lemma mer4[thy_expl]: "sorted2 (t # ts) \<and> \<not> t \<le> r \<Longrightarrow> sorted2 (r # (merge (t#ts) []))" by simp
 
-lemma mer4': "sorted' (t # ts) \<and> t \<le> r \<Longrightarrow> sorted' (t # merge ts [r])"
+lemma mer4'[thy_expl]: "sorted2 (t # ts) \<and> t \<le> r \<Longrightarrow> sorted2 (t # merge ts [r])"
 by (hipster_induct_schemes merge.simps mer3)
 
-lemma mer5': "sorted' (t # ts) \<and> r \<le> v \<and> \<not> t \<le> r \<Longrightarrow> sorted' (r # (merge (t#ts) [v]))"
-(*apply(induction ts rule: sorted'.induct)
+lemma mer5'[thy_expl]: "sorted2 (t # ts) \<and> r \<le> v \<and> \<not> t \<le> r \<Longrightarrow> sorted2 (r # (merge (t#ts) [v]))"
+(*apply(induction ts rule: sorted2.induct)
 apply(simp_all add: mer4 mer3 mer2 mer1)
-apply(metis sorted'.simps merge.simps)*)
+apply(metis sorted2.simps merge.simps)*)
 by (hipster_induct_schemes merge.simps mer3)
 
-lemma mer5'': "sorted' (r # rs) \<and> \<not> t \<le> r \<Longrightarrow> sorted' (r # (merge [t] rs))"
-by (hipster_induct_schemes sorted'.simps)
+lemma mer5''[thy_expl]: "sorted2 (r # rs) \<and> \<not> t \<le> r \<Longrightarrow> sorted2 (r # (merge [t] rs))"
+by (hipster_induct_schemes sorted2.simps)
 
-lemma ssu: "sorted' (r # rs) \<and> t \<le> r \<Longrightarrow> sorted' (t # (merge [] (r#rs)))" by (metis merge.simps sorted'.simps)
+lemma ssu[thy_expl]: "sorted2 (r # rs) \<and> t \<le> r \<Longrightarrow> sorted2 (t # (merge [] (r#rs)))" by (metis merge.simps sorted2.simps)
 (*by (hipster_induct_simp_metis)*)
 
-lemma ssu': "sorted' (r # rs) \<and> t \<le> v \<and> t \<le> r \<Longrightarrow> sorted' (t # (merge [v] (r#rs)))"
-by (metis mer5'' merge.simps sorted'.simps)
-lemma ssu'': " sorted' [t, v] \<and> sorted' (r # rs) \<and> t \<le> r \<Longrightarrow> sorted' (t # (merge [v] (r#rs)))"
-(*by (metis sorted'.simps(3) ssu')*)
-by (hipster_induct_schemes sorted'.simps mer5'')
+lemma ssu'[thy_expl]: "sorted2 (r # rs) \<and> t \<le> v \<and> t \<le> r \<Longrightarrow> sorted2 (t # (merge [v] (r#rs)))"
+by (metis mer5'' merge.simps sorted2.simps)
+lemma ssu''[thy_expl]: " sorted2 [t, v] \<and> sorted2 (r # rs) \<and> t \<le> r \<Longrightarrow> sorted2 (t # (merge [v] (r#rs)))"
+(*by (metis sorted2.simps(3) ssu')*)
+by (hipster_induct_schemes sorted2.simps mer5'')
+
+lemma cons1[thy_expl]: "sorted2 (t # ts) \<Longrightarrow> sorted2 ts"
+by hipster_induct_simp_metis
+(*by (metis sorted2.elims(3) sorted2.simps(3))*)
+
+lemma t1 : "sorted2 ts \<and> ts \<noteq> [] \<and> t \<le> hd ts \<Longrightarrow> sorted2 (t # ts)"
+by hipster_induct_simp_metis
+(*by (metis list.sel sorted2.elims(3))*)
+
+lemma mer6[thy_expl]: "(sorted2 ts \<and> ts \<noteq> [] \<and> sorted2 (r # rs)) \<Longrightarrow> (sorted2 ((merge ts (r#rs))))"
+apply(induction ts rule: sorted2.induct)
+apply(induction rs rule: sorted2.induct)
+apply(simp_all only: thy_expl)
+apply(simp add: ssu'')
+apply(rule conjI)
+apply(rule impI)
+apply(simp add: thy_expl)
+apply(rule impI)
+apply(rule conjI)
+apply(simp add: thy_expl)
+apply(simp add: thy_expl)
+by (hipster_induct_schemes ssu' ssu'' mer5' mer5'' mer3)
+sledgehammer
+apply(metis sorted2.simps ssu'' mer3 ssu ssu' mer4 mer2 mer1 t1 mer5' mer5'' mer4')
 
 (* simplification can very much screw up the goal state! *)
-lemma mer5: "(sorted' (t # ts) \<and> sorted' (r # rs) \<and> t \<le> r) \<Longrightarrow> (sorted' (t # (merge ts (r#rs))))"
-apply(induction ts rule: sorted'.induct)
+lemma mer5[thy_expl]: "(sorted2 (t # ts) \<and> sorted2 (r # rs) \<and> t \<le> r) \<Longrightarrow> (sorted2 (t # (merge ts (r#rs))))"
+apply(induction ts rule: sorted2.induct)
 apply(simp)
 apply(simp add: mer5'')
 apply(simp add: mer4' mer5'' mer3 ssu' ssu'' ssu)
@@ -88,44 +112,39 @@ apply(rule impI, rule conjI)
 apply(simp_all)
 apply(drule conjE)
 apply(simp_all add: ssu' mer5'' mer4 mer4' mer3 mer2 mer1 ssu'' mer5')
-
-apply (metis (full_types) sorted'.simps merge.simps if_splits list.exhaust list.distinct)
-apply(simp add: ssu ssu' mer3 mer2 mer1 ssu'' mer5' mer4')
+(*apply (metis (full_types) sorted2.simps merge.simps if_splits list.exhaust list.distinct)*)
+(*apply(simp add: ssu ssu' mer3 mer2 mer1 ssu'' mer5' mer4')*)
  (*
 apply(metis merge.simps(3) mer5' mer4' mer3 mer4)*)
 sorry
 
-lemma cons1: "sorted' (t # ts) \<Longrightarrow> sorted' ts"
-by hipster_induct_simp_metis
-(*by (metis sorted'.elims(3) sorted'.simps(3))*)
-
-lemma mergeS: "sorted' ts \<and> sorted' rs \<Longrightarrow> sorted' (merge ts rs)"
+lemma mergeS: "sorted2 ts \<and> sorted2 rs \<Longrightarrow> sorted2 (merge ts rs)"
 apply(induction ts rs rule: merge.induct)
 apply(simp_all add: mer1 mer2)
-by (metis mer4 mer5 merge.simps sorted'.simps)
+by (metis mer4 mer5 merge.simps sorted2.simps)
 (*
 apply(cases rs)
 apply(simp_all)
-by (hipster_induct_schemes mer1 mer5'' mer5 merge.simps sorted'.simps)*)
-(*apply(induction ts rule: sorted'.induct)
+by (hipster_induct_schemes mer1 mer5'' mer5 merge.simps sorted2.simps)*)
+(*apply(induction ts rule: sorted2.induct)
 apply(simp add: mer1)
 apply(simp add: mer5'')
-by (metis mer4 mer5 merge.simps sorted'.simps)*)
-(* apply(induction ts rule: sorted'.induct)
+by (metis mer4 mer5 merge.simps sorted2.simps)*)
+(* apply(induction ts rule: sorted2.induct)
 apply(simp add: mer1)
 apply(simp add: mer2)
 apply(cases rs)
 apply(simp_all)
-by (metis mer4 mer5 merge.simps sorted'.simps)*)
+by (metis mer4 mer5 merge.simps sorted2.simps)*)
 (*   by (induct xs ys rule: merge.induct) (auto simp add: ball_Un not_le less_le sorted_Cons) *)
 
-lemma smsort: "sorted' (msort xs)"
+lemma smsort: "sorted2 (msort xs)"
 by (hipster_induct_schemes mergeS)
 
-(*lemma merComm: "sorted' ts \<and> sorted' rs \<Longrightarrow> merge rs ts = merge ts rs"
+(*lemma merComm: "sorted2 ts \<and> sorted2 rs \<Longrightarrow> merge rs ts = merge ts rs"
 apply(induction rs ts rule: merge.induct)
 apply(simp_all)
-apply(metis sorted'.cases merge.simps(1) merge.simps(2))*)
+apply(metis sorted2.cases merge.simps(1) merge.simps(2))*)
 
 
 
